Added Withdraw mechanic

verification/src/launchpad.dfy
@@ -276,5 +276,50 @@ module Launchpad {
                            );
         (newContract, newAmount, newWeight, newRefund)
     }
+
+    /*
+        function WithdrawSpec(intentAccount: IntentAccount, amount: nat, time: nat)
+          : (AuroraLaunchpadContract)
+          requires Valid()
+          requires intentAccount in investments
+          requires amount > 0
+          requires var status := GetStatus(time);
+                   (config.mechanic.PriceDiscovery? && status == LaunchpadStatus.Ongoing) ||
+                   status == LaunchpadStatus.Failed ||
+                   status == LaunchpadStatus.Locked
+          requires var investment := investments[intentAccount];
+                   match config.mechanic {
+                     case FixedPrice(_, _) => amount == investment.amount
+                     case PriceDiscovery   => amount <= investment.amount
+                   }
+          ensures var newContract := WithdrawSpec(intentAccount, amount, time);
+                  var oldInvestment := investments[intentAccount];
+                  var (expectedNewInvestment, expectedNewTotalSoldTokens) := W.WithdrawSpec(config, oldInvestment, amount, totalSoldTokens, time);
+                  newContract.totalDeposited == totalDeposited - amount &&
+                  newContract.totalSoldTokens == expectedNewTotalSoldTokens &&
+                  newContract.investments[intentAccount] == expectedNewInvestment &&
+                  newContract.config == config &&
+                  newContract.isSaleTokenSet == isSaleTokenSet &&
+                  newContract.isLocked == isLocked &&
+                  newContract.accounts == accounts &&
+                  newContract.participantsCount == participantsCount
+        {
+            var investment := investments[intentAccount];
+            var (newInvestment, newTotalSoldTokens) :=
+                W.WithdrawSpec(config, investment, amount, totalSoldTokens, time);
+            var newTotalDeposited := if totalDeposited >= amount then totalDeposited - amount else 0;
+            var newInvestments := investments[intentAccount := newInvestment];
+            AuroraLaunchpadContract(
+                config,
+                newTotalDeposited,
+                newTotalSoldTokens,
+                isSaleTokenSet,
+                isLocked,
+                accounts,
+                participantsCount,
+                newInvestments
+            )
+        }
+    */
   }
 }
